progs/verif_threaded_counter.v
@@ -7,10 +7,12 @@ Local Open Scope logic.
 Instance CompSpecs : compspecs.
 Proof. make_compspecs prog. Defined.  
 
-Definition t_struct_mutex1 := Tstruct _ctr_mutex noattr.
+Definition t_struct_mutex1 := Tstruct _ctr_lock noattr.
 
 Definition t_struct_zero := Tstruct _zero noattr.
 Definition t_struct_ctr := Tstruct _ctr noattr.
+
+(* Sequential stuff *)
 
 Definition reset_spec :=
  DECLARE _reset
@@ -41,16 +43,132 @@ Definition incr_spec :=
   WITH z : int, addof_ctr: val, ctr: val
   PRE  [] 
         PROP ()
-        LOCAL()
-        SEP()
+        LOCAL(gvar _ctr addof_ctr)
+        SEP(`(data_at Ews tint (repinj tint z) ctr);`(data_at Ews (tptr tint) ctr addof_ctr))
   POST [tvoid]
         PROP()
         LOCAL()
-        SEP().
+        SEP(`(data_at Ews tint (repinj tint (Int.add z Int.one)) ctr);`(data_at Ews (tptr tint) ctr addof_ctr)).
+
+Definition counter_funspecs : funspecs :=
+  reset_spec ::
+(*  freelock_spec :: *)
+  incr_spec ::
+  read_spec ::
+  (*  exit_thread_spec ::*)
+  nil.
+
+
+(* Threads specifications*)
+
+Definition tlock := Tstruct _lock_t noattr.
+Axiom lock_inv : share -> val -> mpred -> mpred.
+Parameter Rlock_placeholder : mpred.
+Parameter spawned_precondition_placeholder : val -> mpred.
+Definition voidstar_funtype :=
+  Tfunction
+    (Tcons (tptr tvoid) Tnil)
+    (tptr tvoid)
+    cc_default.
+
+Definition makelock_spec :=
+  DECLARE _makelock
+   WITH v : val, sh : share
+   PRE [ _ctr_lock OF tptr tlock ]
+     PROP (writable_share sh)
+     LOCAL (temp _ctr_lock v)
+     (* SEP (`(mapsto_ Tsh tlock v)) *)  (* ask andrew: that, or mapsto ... (default_val tlock) ? *)
+     SEP (`(data_at_ Tsh tlock v))
+   POST [ tvoid ]
+     PROP ()
+     LOCAL ()
+     SEP (`(lock_inv Tsh v Rlock_placeholder)).
+
+Definition acquire_spec :=
+  DECLARE _acquire
+   WITH v : val, sh : share
+   PRE [ _ctr_lock OF tptr tlock ]
+     PROP (readable_share sh)
+     LOCAL (temp _ctr_lock v)
+     SEP (`(lock_inv sh v Rlock_placeholder))
+   POST [ tvoid ]
+     PROP ()
+     LOCAL ()
+     SEP (`(lock_inv sh v Rlock_placeholder) ; `Rlock_placeholder).
+
+Definition release_spec :=
+  DECLARE _release
+   WITH v : val, sh : share
+   PRE [ _ctr_lock OF tptr tlock ]
+     PROP (readable_share sh)
+     LOCAL (temp _ctr_lock v)
+     SEP (`(lock_inv sh v Rlock_placeholder) ; `Rlock_placeholder)
+   POST [ tvoid ]
+     PROP ()
+     LOCAL ()
+     SEP (`(lock_inv sh v Rlock_placeholder)).
+
+Definition spawn_thread_spec := (* universe inconsistency if "WITH P" *)
+  DECLARE _spawn_thread
+   WITH f : val, b : val
+   PRE [_thread_func OF tptr voidstar_funtype, _thread_mutex OF tptr tvoid]
+     PROP ()
+     LOCAL (temp _thread_mutex b)
+     SEP ((EX _y : ident,
+     `(func_ptr'
+       (WITH y : val
+        PRE [ _y OF tptr tvoid ]
+          PROP  ()
+          LOCAL (temp _y y)
+          SEP   (`(spawned_precondition_placeholder y))
+        POST [tvoid]
+          PROP  ()
+          LOCAL ()
+          SEP   (emp)
+       )
+       f)) ; `(spawned_precondition_placeholder b))
+   POST [ tvoid ]
+     PROP  ()
+     LOCAL ()
+     SEP   (emp).
+
+Definition threads_funspecs : funspecs :=
+  makelock_spec ::
+(*  freelock_spec :: *)
+  acquire_spec ::
+  release_spec ::
+  spawn_thread_spec ::
+  (*  exit_thread_spec ::*)
+  nil.
+
+(* Threaded part*)
+Definition concurrent_incr_spec :=
+  DECLARE _concurrent_incr
+   WITH  addof_ctr_lock: val, addof_ctr: val,v : val, sh : share
+   PRE [ ]
+     PROP (readable_share sh) (*Holds partial ownerchip of ctr lock*)
+     LOCAL (gvar _ctr addof_ctr; gvar _ctr_lock addof_ctr_lock; gvar _ctr_lock v)
+     SEP (`(lock_inv sh v Rlock_placeholder))
+   POST [ tvoid ]
+     PROP ()
+     LOCAL ()
+     SEP ().
+
+Definition thread_func_spec :=
+  DECLARE _thread_func
+   WITH z: int
+   PRE [ ]
+     PROP () (*Holds partial ownerchip of two locks*)
+     LOCAL ()
+     SEP ()
+   POST [ tvoid ]
+     PROP ()
+     LOCAL ()
+     SEP ().
 
 Definition main_spec :=
  DECLARE _main
-  WITH z0 : int, z1 : int, addof_ctr: val, ctr: val
+  WITH  z0 : int, z1 : int, addof_ctr: val, ctr: val
   PRE  [] 
         PROP ()
         LOCAL(gvar _ctr addof_ctr)
@@ -60,27 +178,89 @@ Definition main_spec :=
         LOCAL( temp ret_temp (Vint (Int.repr 2)))
         SEP(`(data_at Ews tint (repinj tint z1) ctr);`(data_at Ews (tptr tint) ctr addof_ctr)).
 
-Definition Vprog : varspecs := (_ctr_mutex, )::(_ctr, tptr tint)::(_zero,tint)::nil.
+Definition Vprog : varspecs := (_ctr_lock, tlock)::(_ctr, tptr tint)::(_zero,tint)::nil.
 
-Definition Gprog : funspecs := 
-  reset_spec::incr_spec::read_spec::main_spec::nil.
+Definition Gprog : funspecs :=
+  counter_funspecs ++ threads_funspecs ++ concurrent_incr_spec:: thread_func_spec::main_spec::nil.
 
-Definition main_spec :=
- DECLARE _main
-  WITH z : int, addof_ctr: val, ctr: val
-  PRE  [] 
-        PROP ()
-        LOCAL(gvar _counter addof_ctr)
-        SEP(`(data_at Ews tint (repinj tint z) ctr);`(data_at Ews (tptr tint) ctr addof_ctr))
-  POST [tint]
-        PROP()
-        LOCAL( temp ret_temp (Vint (Int.one)))
-        SEP(`(data_at Ews tint (repinj tint z) ctr);`(data_at Ews (tptr tint) ctr addof_ctr)).
 
-Definition Vprog : varspecs := (_counter, tptr tint)::nil.
+(*Lets do this first:*)
+Lemma body_concurrent_incr:  semax_body Vprog Gprog f_concurrent_incr concurrent_incr_spec.
+  start_function.
+  forward _ctr_lock_ptr.
+  forward_call' (v, sh) r.
+  forward_call' (_ctr_lock_ptr).
+ 
+ forward thread_mutex_ptr_.
+ forward.
 
-Definition Gprog : funspecs := 
-  main_spec::nil.
+Proof.
+
+Lemma body_incr:  semax_body Vprog Gprog f_incr incr_spec.
+Proof.
+ start_function.
+ name ctr_ _ctr.
+ name ctr0_ _ctr0.
+ name t_ _t.
+ forward.
+ forward.
+ forward.
+ forward.
+unfold_repinj.
+cancel.
+apply derives_refl'. unfold data_at. f_equal. f_equal. f_equal.
+unfold unfold_reptype'. simpl.
+rewrite <- eq_rect_eq.
+auto.
+Qed.
+
+Lemma body_reset:  semax_body Vprog Gprog f_reset reset_spec.
+Proof.
+ start_function.
+ name ctr_ _ctr.
+ name ctr0_ _ctr0.
+ name t_ _t.
+ forward.
+ forward.
+ forward.
+unfold_repinj.
+cancel.
+Qed.
+
+
+Lemma body_read:  semax_body Vprog Gprog f_read read_spec.
+Proof.
+ start_function.
+ name ctr_ _ctr.
+ name ctr0_ _ctr0.
+ name t_ _t.
+ forward.
+ forward.
+ forward. 
+ unfold_repinj.
+ apply andp_right; cancel.
+ apply prop_right.
+ revert H0; unfold_repinj. congruence.
+Qed.
+
+
+(*Threaded part*)
+Lemma body_concurrent_incr:  semax_body Vprog Gprog f_concurrent_incr concurrent_incr_spec.
+  start_function.
+  forward_call' (_ctr_lock).
+ 
+ forward thread_mutex_ptr_.
+ forward.
+
+Proof.
+
+Lemma body_thread_incr:  semax_body Vprog Gprog f_thread_func thread_func_spec.
+ start_function.
+ forward thread_mutex_ptr_.
+ forward.
+
+Proof.
+
 
 Lemma body_main:  semax_body Vprog Gprog f_main main_spec.
 Proof.
